Main.lean
@@ -1,5 +1,7 @@
 import Linen.Data.Json
+import Linen.System.Console.Ansi
 
+open System.Console.Ansi
 
 def main : IO Unit :=
-  IO.println s!"Hello, {Data.Json.Value.null.isNull}!"
+  IO.println $ setFg .red ++ s!"Hello, {Data.Json.Value.null.isNull}!"
